refactor inhale acc rel atomic rule to handle the temporary variable assignment separately

InhaleRel.thy
@@ -1,5 +1,5 @@
 theory InhaleRel
-  imports ExpRel ExprWfRel TotalViper.ViperBoogieTranslationInterface Simulation
+  imports ExpRel ExprWfRel TotalViper.ViperBoogieTranslationInterface Simulation SimulationInstUtil
 begin
 
 definition inhale_rel ::
@@ -164,19 +164,14 @@ definition inhale_acc_normal_premise
        (let W' = (if r = Null then {\<omega>} else inhale_perm_single StateCons \<omega> (the_address r,f) (Some (Abs_prat p))) in
        (W' \<noteq> {} \<and> \<omega>' \<in> W'))"
 
-definition pos_perm_rel
-  where "pos_perm_rel R R' ctxt_vpr StateCons P ctxt e_p p \<gamma>2 \<gamma>3   = 
-     rel_general R R'
-                  (\<lambda> \<omega> \<omega>'. \<omega> = \<omega>' \<and> (ctxt_vpr, StateCons, Some \<omega> \<turnstile> \<langle>e_p;\<omega>\<rangle> [\<Down>]\<^sub>t (Val (VPerm p)) \<and> p \<ge> 0))
-                  (\<lambda> \<omega>. (ctxt_vpr, StateCons, Some \<omega> \<turnstile> \<langle>e_p;\<omega>\<rangle> [\<Down>]\<^sub>t (Val (VPerm p)) \<and> p < 0))
-                  P ctxt \<gamma>2 \<gamma>3"
-
 lemma inhale_rel_field_acc:
   assumes 
     WfRcv: "expr_wf_rel (state_rel_ext R) ctxt_vpr StateCons P ctxt e_rcv_vpr \<gamma> \<gamma>1" and
-    WfPerm: "expr_wf_rel (state_rel_ext R) ctxt_vpr StateCons P ctxt e_p \<gamma>1 \<gamma>2" and
-  
-    PosPermRel:  "\<And>p. pos_perm_rel R (R' p) ctxt_vpr StateCons P ctxt e_p p \<gamma>2 \<gamma>3" and
+    WfPerm: "expr_wf_rel (state_rel_ext R) ctxt_vpr StateCons P ctxt e_p \<gamma>1 \<gamma>2" and 
+    PosPermRel:  "\<And>p. rel_general R (R' p)
+                  (\<lambda> \<omega> \<omega>'. \<omega> = \<omega>' \<and> (ctxt_vpr, StateCons, Some \<omega> \<turnstile> \<langle>e_p;\<omega>\<rangle> [\<Down>]\<^sub>t (Val (VPerm p)) \<and> p \<ge> 0))
+                  (\<lambda> \<omega>. (ctxt_vpr, StateCons, Some \<omega> \<turnstile> \<langle>e_p;\<omega>\<rangle> [\<Down>]\<^sub>t (Val (VPerm p)) \<and> p < 0))
+                  P ctxt \<gamma>2 \<gamma>3" and
      UpdInhRel: "\<And>p r. rel_general (R' p) R
                   (\<lambda> \<omega> \<omega>'. inhale_acc_normal_premise ctxt_vpr StateCons e_rcv_vpr f e_p p r \<omega> \<omega>')
                   (\<lambda> \<omega>. False) P ctxt \<gamma>3 \<gamma>'" \<comment>\<open>Here, the simulation needs to revert back to R\<close>
@@ -215,7 +210,7 @@ proof (rule inhale_rel_intro_2)
         by presburger
     
       from InhAcc \<open>0 \<le> p\<close> obtain ns3 where "red_ast_bpl P ctxt (\<gamma>, Normal ns) (\<gamma>3, Normal ns3)" and "R' p \<omega> ns3" 
-        using rel_success_elim[OF HOL.iffD1[OF pos_perm_rel_def PosPermRel] \<open>R \<omega> ns2\<close>] Red2 red_ast_bpl_transitive
+        using rel_success_elim[OF PosPermRel \<open>R \<omega> ns2\<close>] Red2 red_ast_bpl_transitive
         by blast
 
       thus "\<exists>ns'. red_ast_bpl P ctxt (\<gamma>, Normal ns) (\<gamma>', Normal ns') \<and> R \<omega>' ns'"
@@ -229,7 +224,7 @@ proof (rule inhale_rel_intro_2)
         by fastforce
 
       with InhAcc show "\<exists>c'. red_ast_bpl P ctxt (\<gamma>, Normal ns) c' \<and> snd c' = Failure"
-        using rel_failure_elim[OF HOL.iffD1[OF pos_perm_rel_def PosPermRel] \<open>R \<omega> ns2\<close>] Red2 red_ast_bpl_transitive
+        using rel_failure_elim[OF PosPermRel \<open>R \<omega> ns2\<close>] Red2 red_ast_bpl_transitive
         by blast
     qed
   next 
@@ -258,104 +253,100 @@ proof (rule inhale_rel_intro_2)
   qed
 qed
 
-definition pred_eq
-  where "pred_eq x v = (x = v)"
-
-\<comment>\<open>Factor out temporary variable\<close>
-lemma pos_perm_rel:
-  assumes 
-            StateRel: "\<And> \<omega> ns. R \<omega> ns \<Longrightarrow> state_rel Pr TyRep Tr AuxPred ctxt \<omega> ns" and
-ExpRel: "exp_rel_vpr_bpl (state_rel_ext R) ctxt_vpr ctxt e_p e_p_bpl" and
+lemma pos_perm_rel_1:
+  assumes
+  StateRel: "state_rel Pr TyRep Tr AuxPred ctxt \<omega> ns" (is "?R \<omega> ns") and
+  RedPerm:  "ctxt_vpr, StateCons, Some \<omega> \<turnstile> \<langle>e_p;\<omega>\<rangle> [\<Down>]\<^sub>t Val (VPerm p)" and
+  ExpRel: "exp_rel_vpr_bpl (state_rel_ext (state_rel Pr TyRep Tr AuxPred ctxt)) ctxt_vpr ctxt e_p e_p_bpl" and
          DisjAux: "temp_perm \<notin> {heap_var Tr, mask_var Tr} \<union> ran (var_translation Tr) \<union> 
                      ran (field_translation Tr) \<union> range (const_repr Tr) \<union> dom AuxPred" and
          LookupTyTemp: "lookup_var_ty (var_context ctxt) temp_perm = Some (TPrim TReal)" and
-         TyInterp:  "type_interp ctxt = vbpl_absval_ty TyRep" and
-         WritePermConst: "zero_perm = const_repr Tr CNoPerm"
+         TyInterp:  "type_interp ctxt = vbpl_absval_ty TyRep"
+   shows "\<exists>ns'. red_ast_bpl P ctxt (((BigBlock name (Lang.Assign temp_perm e_p_bpl # cs) s tr), cont), Normal ns)
+                                   ((BigBlock name cs s tr, cont), Normal ns') \<and>
+                (state_rel Pr TyRep Tr (AuxPred(temp_perm \<mapsto> pred_eq (RealV (real_of_rat p)))) ctxt \<omega> ns')"
+           (is "\<exists>ns'. ?red ns' \<and> ?R' \<omega> ns'")
+proof (rule exI, rule conjI)
+  let ?p_bpl = "RealV (real_of_rat p)"
 
-\<comment>\<open>TODO: handle case e_p is statically determined to be non-negative
-         factor out temporary variable assignment\<close>
-shows "pos_perm_rel R 
-         (state_rel Pr TyRep Tr (AuxPred(temp_perm \<mapsto> pred_eq (RealV (real_of_rat p)))) ctxt) 
-         ctxt_vpr StateCons P ctxt e_p p 
-         ((BigBlock name (Lang.Assign temp_perm e_p_bpl # Assert ((Var temp_perm) \<guillemotleft>Ge\<guillemotright> (Var zero_perm)) # cs) s tr), cont) 
-         (BigBlock name cs s tr, cont)" (is "pos_perm_rel R ?R' ctxt_vpr StateCons P ctxt e_p p ?\<gamma> ?\<gamma>'")
-  unfolding pos_perm_rel_def
+  from RedPerm have RedPermBpl: "red_expr_bpl ctxt e_p_bpl ns ?p_bpl"
+    using exp_rel_vpr_bpl_elim[OF ExpRel] \<open>?R \<omega> ns\<close>
+    by (metis val_rel_vpr_bpl.simps(5))
+
+  let ?ns' = "update_var (var_context ctxt) ns temp_perm ?p_bpl"
+
+  have StateRel2: "state_rel Pr TyRep Tr (AuxPred(temp_perm \<mapsto> pred_eq ?p_bpl)) ctxt \<omega> ?ns'"
+    using state_rel_new_auxvar[OF \<open>?R \<omega> ns\<close> DisjAux _ TyInterp LookupTyTemp]
+    unfolding pred_eq_def
+    by simp
+
+  show "?red ?ns'"
+    apply (rule red_ast_bpl_one_simple_cmd)
+    by (fastforce intro!: RedAssign LookupTyTemp RedPermBpl)
+
+  show "?R' \<omega> ?ns'"
+    using StateRel2
+    by blast
+qed
+
+lemma pos_perm_rel_2:
+
+\<comment>\<open>TODO: handle case e_p is statically determined to be non-negative\<close>
+assumes  WritePermConst: "zero_perm = const_repr Tr CNoPerm"
+
+shows "rel_general (state_rel Pr TyRep Tr (AuxPred(temp_perm \<mapsto> pred_eq (RealV (real_of_rat p)))) ctxt)
+                   (state_rel Pr TyRep Tr (AuxPred(temp_perm \<mapsto> pred_eq (RealV (real_of_rat p)))) ctxt)
+     (\<lambda>\<omega> \<omega>'. \<omega> = \<omega>' \<and> ctxt_vpr, StateCons, Some \<omega> \<turnstile> \<langle>e_p;\<omega>\<rangle> [\<Down>]\<^sub>t Val (VPerm p) \<and> 0 \<le> p)
+     (\<lambda>\<omega>. ctxt_vpr, StateCons, Some \<omega> \<turnstile> \<langle>e_p;\<omega>\<rangle> [\<Down>]\<^sub>t Val (VPerm p) \<and> p < 0) P ctxt
+     (BigBlock name (cmd.Assert (expr.Var temp_perm \<guillemotleft>Ge\<guillemotright> expr.Var zero_perm) # cs) s tr, cont)
+     (BigBlock name cs s tr, cont)" (is "rel_general ?R ?R ?Success ?Fail P ctxt ?\<gamma> ?\<gamma>'")
 proof (rule rel_intro)
   fix \<omega> ns \<omega>'
-  assume "R \<omega> ns" and
+  assume "?R \<omega> ns" and
          A: "\<omega> = \<omega>' \<and> ctxt_vpr, StateCons, Some \<omega> \<turnstile> \<langle>e_p;\<omega>\<rangle> [\<Down>]\<^sub>t Val (VPerm p) \<and> 0 \<le> p"
-  from this have
-    RedPerm:  "ctxt_vpr, StateCons, Some \<omega> \<turnstile> \<langle>e_p;\<omega>\<rangle> [\<Down>]\<^sub>t Val (VPerm p)" and "0 \<le> p" 
-    by auto
 
-  note StateRelInst = StateRel[OF \<open>R \<omega> ns\<close>]
-  let ?p_bpl = "real_of_rat p"
+  let ?p_bpl = "RealV (real_of_rat p)"
 
-  from RedPerm have RedPermBpl: "red_expr_bpl ctxt e_p_bpl ns (RealV ?p_bpl)"
-    using exp_rel_vpr_bpl_elim[OF ExpRel] \<open>R \<omega> ns\<close>
-    by (metis val_rel_vpr_bpl.simps(5))
-
-  let ?ns' = "update_var (var_context ctxt) ns temp_perm (RealV ?p_bpl)"
-
-  have StateRelInst2: "state_rel Pr TyRep Tr (AuxPred(temp_perm \<mapsto> pred_eq (RealV ?p_bpl))) ctxt \<omega> ?ns'"
-    using state_rel_new_auxvar[OF StateRelInst DisjAux _ TyInterp LookupTyTemp]
+  have LookupTempPerm: "lookup_var (var_context ctxt) ns temp_perm = Some ?p_bpl"
+    using state_rel_aux_pred_sat_lookup_2[OF \<open>?R \<omega> ns\<close>]
     unfolding pred_eq_def
-    by simp
+    by (metis (full_types) fun_upd_same)
 
-  moreover have "red_ast_bpl P ctxt
-              (?\<gamma>, Normal ns)
-              ((BigBlock name (Assert ((Var temp_perm) \<guillemotleft>Ge\<guillemotright> (Var zero_perm)) # cs) s tr, cont), Normal ?ns')"
-      (is "red_ast_bpl P ctxt _ (?\<gamma>'',_)")
+  have "red_ast_bpl P ctxt (?\<gamma>, Normal ns) (?\<gamma>', Normal ns)"
     apply (rule red_ast_bpl_one_simple_cmd)
-    by (fastforce intro!: RedAssign LookupTyTemp RedPermBpl)
-
-  moreover have "red_ast_bpl P ctxt (?\<gamma>'', Normal ?ns') (?\<gamma>', Normal ?ns')"
-    apply (rule red_ast_bpl_one_simple_cmd)
-    using \<open>0 \<le> p\<close>
+    using A
     by (auto intro!: RedAssertOk Semantics.RedBinOp Semantics.RedVar 
-                        boogie_const_rel_lookup[OF state_rel0_boogie_const[OF state_rel_state_rel0[OF StateRelInst2]]] 
+                        boogie_const_rel_lookup[OF state_rel0_boogie_const[OF state_rel_state_rel0[OF \<open>?R \<omega> ns\<close>]]] 
+             intro: LookupTempPerm
                 simp: \<open>zero_perm = _\<close>)
 
-  ultimately show "\<exists>ns'. red_ast_bpl P ctxt (?\<gamma>, Normal ns) ((BigBlock name cs s tr, cont), Normal ns') \<and>                         
-                              state_rel Pr TyRep Tr (AuxPred(temp_perm \<mapsto> pred_eq (RealV (real_of_rat p)))) ctxt \<omega>' ns'"
-    using RedPerm red_ast_bpl_transitive A
-    by fast
+  thus "\<exists>ns'. red_ast_bpl P ctxt (?\<gamma>, Normal ns) (?\<gamma>', Normal ns') \<and>                         
+                              state_rel Pr TyRep Tr (AuxPred(temp_perm \<mapsto> pred_eq ?p_bpl)) ctxt \<omega>' ns'"
+    using \<open>?R \<omega> ns\<close> A
+    by fast        
 next
   fix \<omega> ns
-  assume "R \<omega> ns"
+  assume "?R \<omega> ns"
   assume "ctxt_vpr, StateCons, Some \<omega> \<turnstile> \<langle>e_p;\<omega>\<rangle> [\<Down>]\<^sub>t Val (VPerm p) \<and> p < 0"
-  from this have RedPerm: "ctxt_vpr, StateCons, Some \<omega> \<turnstile> \<langle>e_p;\<omega>\<rangle> [\<Down>]\<^sub>t Val (VPerm p)" and "p < 0" 
+  from this have "p < 0" 
     by auto
 
-  note StateRelInst = StateRel[OF \<open>R \<omega> ns\<close>]
-  let ?p_bpl = "real_of_rat p"
+  let ?p_bpl = "RealV (real_of_rat p)"
 
-  from RedPerm have RedPermBpl: "red_expr_bpl ctxt e_p_bpl ns (RealV ?p_bpl)"
-    using exp_rel_vpr_bpl_elim[OF ExpRel] \<open>R \<omega> ns\<close>
-    by (metis val_rel_vpr_bpl.simps(5))
-
-  let ?ns' = "update_var (var_context ctxt) ns temp_perm (RealV ?p_bpl)"
-
-  have StateRelInst2: "state_rel Pr TyRep Tr (AuxPred(temp_perm \<mapsto> pred_eq (RealV ?p_bpl))) ctxt \<omega> ?ns'"
-    using  state_rel_new_auxvar[OF StateRelInst DisjAux _ TyInterp LookupTyTemp]
+  have LookupTempPerm: "lookup_var (var_context ctxt) ns temp_perm = Some ?p_bpl"
+    using state_rel_aux_pred_sat_lookup_2[OF \<open>?R \<omega> ns\<close>]
     unfolding pred_eq_def
-    by simp
-  
-  moreover have "red_ast_bpl P ctxt
-              (?\<gamma>, Normal ns)
-              ((BigBlock name (Assert ((Var temp_perm) \<guillemotleft>Ge\<guillemotright> (Var zero_perm)) # cs) s tr, cont), Normal ?ns')"
-      (is "red_ast_bpl P ctxt _ (?\<gamma>'',_)")
-    apply (rule red_ast_bpl_one_simple_cmd)
-    by (fastforce intro!: RedAssign LookupTyTemp RedPermBpl)
+    by (metis (full_types) fun_upd_same)
 
-  moreover have "red_ast_bpl P ctxt (?\<gamma>'', Normal ?ns') (?\<gamma>', Failure)"
+  have "red_ast_bpl P ctxt (?\<gamma>, Normal ns) (?\<gamma>', Failure)"
     apply (rule red_ast_bpl_one_simple_cmd)
     using \<open>p < 0\<close>
     by (auto intro!: RedAssertFail Semantics.RedBinOp Semantics.RedVar 
-                        boogie_const_rel_lookup[OF state_rel0_boogie_const[OF state_rel_state_rel0[OF StateRelInst2]]] 
+                        boogie_const_rel_lookup[OF state_rel0_boogie_const[OF state_rel_state_rel0[OF \<open>?R \<omega> ns\<close>]]]
+             intro: LookupTempPerm
                 simp: \<open>zero_perm = _\<close> )
 
-  ultimately show 
+  thus 
        "\<exists>c'. snd c' = Failure \<and> red_ast_bpl P ctxt (?\<gamma>, Normal ns) c'"
     using red_ast_bpl_transitive
     by fastforce
@@ -366,31 +357,38 @@ lemma non_null_receiver_inh_rel:
        InhAccNormal: "inhale_acc_normal_premise ctxt_vpr StateCons e_rcv_vpr f_vpr e_p p r \<omega> \<omega>'" and
  RcvRel: "exp_rel_vpr_bpl (state_rel_ext (state_rel (program_total ctxt_vpr) TyRep Tr (AuxPred(temp_perm \<mapsto> pred_eq (RealV (real_of_rat p)))) ctxt)) 
                           ctxt_vpr ctxt e_rcv_vpr e_rcv_bpl" and
- WritePermConst: "null_const = const_repr Tr CNull"
+ NullConst: "null_const = const_repr Tr CNull" and
+ NoPermConst: "no_perm_const = const_repr Tr CNoPerm"
   shows 
           "\<exists>ns'. red_ast_bpl P ctxt 
-               ( (BigBlock name ((Assume (((Var temp_perm) \<guillemotleft>Gt\<guillemotright> no_perm_const) \<guillemotleft>Imp\<guillemotright> (e_rcv_bpl \<guillemotleft>Neq\<guillemotright> Var null_const))) # cs) str tr, cont) , Normal ns) 
+               ( (BigBlock name ((Assume (((Var temp_perm) \<guillemotleft>Gt\<guillemotright> (Var no_perm_const)) \<guillemotleft>Imp\<guillemotright> (e_rcv_bpl \<guillemotleft>Neq\<guillemotright> Var null_const))) # cs) str tr, cont) , Normal ns) 
                 ( (BigBlock name cs str tr, cont), Normal ns') \<and> 
-                 ?R \<omega> ns'" 
-  sorry
-(*
+                 ?R \<omega> ns'" (is "\<exists>ns'. red_ast_bpl P ctxt (?\<gamma>, Normal ns) (?\<gamma>', Normal ns') \<and> ?R _ _")
 proof (rule exI[where ?x="ns"])
-  from InhAccNormal exp_rel_vpr_bpl_elim_2[OF RcvRel] \<open>?R \<omega> ns\<close> have "red_expr_bpl ctxt e_rcv_bpl ns (AbsV (ARef r))"
+  from InhAccNormal exp_rel_vpr_bpl_elim_2[OF RcvRel] \<open>?R \<omega> ns\<close> have RedRcvBpl: "red_expr_bpl ctxt e_rcv_bpl ns (AbsV (ARef r))"
     unfolding inhale_acc_normal_premise_def
     by (metis val_rel_vpr_bpl.simps(3))
 
-    from \<open>?R \<omega> ns\<close> have LookupTempPerm: "lookup_var (var_context ctxt) ns temp_perm = Some (RealV (real_of_rat p))"
-      using state_rel_aux_pred_sat_lookup_2
-      unfolding pred_eq_def      
-      by (metis (full_types) fun_upd_same)
+  from \<open>?R \<omega> ns\<close> have LookupTempPerm: "lookup_var (var_context ctxt) ns temp_perm = Some (RealV (real_of_rat p))"
+    using state_rel_aux_pred_sat_lookup_2
+    unfolding pred_eq_def      
+    by (metis (full_types) fun_upd_same)
 
-  moreover have "lookup_var (var_context ctxt) ns null_const = Some (AbsV (ARef Null))"
-    using boogie_const_rel_lookup[OF state_rel0_boogie_const[OF state_rel_state_rel0[OF \<open>?R \<omega> ns\<close>]]]
-          \<open>null_const = _\<close>
-    by simp
-*)    
-  
- 
+  from InhAccNormal have "p > 0 \<longrightarrow> r \<noteq> Null"
+    unfolding inhale_acc_normal_premise_def
+    by blast
+
+
+  have "red_ast_bpl P ctxt (?\<gamma>, Normal ns) (?\<gamma>', Normal ns)"
+    apply (rule red_ast_bpl_one_simple_cmd)
+    by (fastforce intro!: Semantics.RedAssumeOk RedVar Semantics.RedBinOp LookupTempPerm boogie_const_rel_lookup[OF state_rel0_boogie_const[OF state_rel_state_rel0[OF \<open>?R \<omega> ns\<close>]]] 
+                 intro: RedRcvBpl
+                 simp: \<open>p > 0 \<longrightarrow> r \<noteq> Null\<close> \<open>null_const = _\<close> \<open>no_perm_const = _\<close>)
+
+  thus "red_ast_bpl P ctxt (?\<gamma>, Normal ns) (?\<gamma>', Normal ns) \<and> ?R \<omega> ns"
+    using StateRel
+    by blast
+qed
 
 lemma upd_inh_rel:
   assumes
